proof/theories/Optimize_ConcatK.v
@@ -627,6 +627,24 @@ Proof.
       exact (H0 (r2 :: rest) ltac:(unfold ltof; cbn; lia) _ _ _ _ _ Erec).
 Qed.
 
+Lemma optimize_rules_concatK_maps : forall rs n d n' d' rs',
+  optimize_rules_concatK n d rs = (n', d', rs') -> sd_maps d' = sd_maps d.
+Proof.
+  induction rs as [rs H0] using (induction_ltof1 _ (@length rule)).
+  intros n d n' d' rs' H.
+  destruct rs as [| r1 [| r2 rest] ].
+  - cbn in H. inversion H; subst; reflexivity.
+  - cbn in H. inversion H; subst; reflexivity.
+  - rewrite optimize_rules_concatK_cons2 in H. cbv zeta in H.
+    destruct (concat_mergeK_pair r1 r2) as [[[[fields row1] row2] body] |] eqn:Em.
+    + destruct (optimize_rules_concatK (S n) _ rest) as [[m'' dd''] rr''] eqn:Erec.
+      inversion H; subst n' d' rs'. clear H.
+      rewrite (H0 rest ltac:(unfold ltof; cbn; lia) _ _ _ _ _ Erec). reflexivity.
+    + destruct (optimize_rules_concatK n d (r2 :: rest)) as [[m'' dd''] rr''] eqn:Erec.
+      inversion H; subst n' d' rs'. clear H.
+      exact (H0 (r2 :: rest) ltac:(unfold ltof; cbn; lia) _ _ _ _ _ Erec).
+Qed.
+
 Lemma optimize_rules_concatK_mono : forall rs n d n' d' rs',
   optimize_rules_concatK n d rs = (n', d', rs') -> n <= n'.
 Proof.
@@ -689,6 +707,14 @@ Proof.
   intros n d c n' d' c' H. unfold optimize_chain_concatK in H.
   destruct (optimize_rules_concatK n d (c_rules c)) as [[m'' dd''] rr''] eqn:E.
   inversion H; subst. apply (optimize_rules_concatK_vmaps _ _ _ _ _ _ E).
+Qed.
+
+Lemma optimize_chain_concatK_maps : forall n d c n' d' c',
+  optimize_chain_concatK n d c = (n', d', c') -> sd_maps d' = sd_maps d.
+Proof.
+  intros n d c n' d' c' H. unfold optimize_chain_concatK in H.
+  destruct (optimize_rules_concatK n d (c_rules c)) as [[m'' dd''] rr''] eqn:E.
+  inversion H; subst. apply (optimize_rules_concatK_maps _ _ _ _ _ _ E).
 Qed.
 
 Lemma optimize_chain_concatK_keys_bound : forall n d c n' d' c' k,
